modules in Cedar.SymCC and Cedar.Thm.SymCC.Data
Signed-off-by: Craig Disselkoen <cdiss@amazon.com>

cedar-lean/Cedar/SymCC/Data.lean
@@ -14,20 +14,22 @@
  limitations under the License.
 -/
 
-import Cedar.Data
+module
+
+public import Cedar.Data
 import Cedar.Spec
 
 /-!
 This file contains generic utility functions shared by `SymCC` modules.
 -/
 
-@[inline] def BitVec.width {n : Nat} (_ : BitVec n) : Nat := n
+@[inline, expose] public def BitVec.width {n : Nat} (_ : BitVec n) : Nat := n
 
-def BitVec.signedMin (n : Nat) : Int := - 2 ^ (n-1)
+public def BitVec.signedMin (n : Nat) : Int := - 2 ^ (n-1)
 
-def BitVec.signedMax (n : Nat) : Int := 2 ^ (n-1) - 1
+public def BitVec.signedMax (n : Nat) : Int := 2 ^ (n-1) - 1
 
-def BitVec.overflows (n : Nat) (i : Int) : Bool :=
+public def BitVec.overflows (n : Nat) (i : Int) : Bool :=
   i < (BitVec.signedMin n) ||
   i > (BitVec.signedMax n)
 
@@ -35,12 +37,12 @@ namespace Cedar.SymCC
 
 open Cedar.Data
 
-abbrev EntityTag (α) := Map String α
+public abbrev EntityTag (α) := Map String α
 
-abbrev EntityTag.mk {α} (entity tag : α) : EntityTag α :=
+public abbrev EntityTag.mk {α} (entity tag : α) : EntityTag α :=
   Map.mk [("entity", entity), ("tag", tag)]
 
-abbrev EntityTag.wf {α} : EntityTag α → Bool
+public abbrev EntityTag.wf {α} : EntityTag α → Bool
   | .mk _ _ => true
   | _       => false
 
